Work on proving the compiler completeness

imp2lp/src/imp2lp/CompileWithVar.v
@@ -9,9 +9,10 @@ Require Import coqutil.Tactics.case_match.
 Import ListNotations.
 
 Inductive var : Type :=
-| name_var : string -> var
-| attr_var : string * string -> var
-| time_var : var .
+| singleton_var : string -> var
+| access_var : string * string -> var
+| attr_var : string -> var
+| time_var : var.
 
 Variant obj : Set :=
   Bobj : bool -> obj | Zobj : Z -> obj | Sobj : string -> obj.
@@ -64,7 +65,8 @@ Definition interp_Sfn (f : Sfn) (l : list obj) : option string :=
 Variant rel : Set :=
   (* Assume no shadowing and and no repeated use of the same variable name,
 so we can use variable names as relation/datalog var names. *)
-  | str_rel : string -> rel (* unary for variables, assuming SSA form *)
+  | str_rel : string -> rel (* unary for variables *)
+  | res_rel : string -> rel (* for the values of mutable variables upon program termination *)
   | nat_rel : nat -> rel
   | blk_rel : nat -> rel
   | ret_rel : rel
@@ -74,8 +76,9 @@ Variant aggregator : Set :=.
 
 Definition var_eqb (x y : var) : bool :=
   match x, y with
-  | name_var x, name_var y => (x =? y)%string
-  | attr_var (x1, x2), attr_var (y1, y2) => (x1 =? y1)%string && (x2 =? y2)%string
+  | singleton_var x, singleton_var y => (x =? y)%string
+  | access_var (x1, x2), access_var (y1, y2) => (x1 =? y1)%string && (x2 =? y2)%string
+  | attr_var x, attr_var y => (x =? y)%string
   | time_var, time_var => true
   | _, _ => false
   end.
@@ -83,7 +86,7 @@ Definition var_eqb (x y : var) : bool :=
 Lemma var_eqb_spec x y : BoolSpec (x = y) (x <> y) (var_eqb x y).
 Proof.
   destruct x, y; simpl; repeat case_match; try (constructor; congruence).
-  1: destruct (s =? s0)%string eqn:E; constructor;
+  1,3: destruct (s =? s0)%string eqn:E; constructor;
   rewrite ?String.eqb_eq, ?String.eqb_neq in *; congruence.
   1: destruct (s =? s1)%string eqn:E1;
   destruct (s0 =? s2)%string eqn:E2; cbn; constructor;
@@ -124,8 +127,8 @@ Section __.
   Local Notation fact := (fact rel var fn).
 
   Section WithVarenv.
-    (* Context {varenv : map.map string rel} {varenv_ok : map.ok varenv}. *)
-    Context {attrenv : map.map (string * string) var} {attrenv_ok : map.ok attrenv}.
+    (* Context {varenv : map.map string rel} {varenv_ok : map.ok varenv}.
+    Context {attrenv : map.map (string * string) var} {attrenv_ok : map.ok attrenv}. *)
     Context {tenv : map.map string type} {tenv_ok : map.ok tenv}.
 
     Context (timestamp_attr singleton_attr: string).
@@ -133,46 +136,44 @@ Section __.
     Section WithTimestamp.
       Context (in_timestamp : dexpr).
 
-      Fixpoint lower_aexpr (m : attrenv) (e : aexpr) : (dexpr * list fact) :=
+      Fixpoint lower_aexpr (e : aexpr) : (dexpr * list fact) :=
         (* Assume no variable shadowing and no reuse of variable names, even across mutable and immutable variables
          m: maps each (row variable, attribute) pair to a datalog variable.
          return (datalog expression, list of clauses assumed for the expression, new threshold for fresh variables *)
         match e with
-        | AVar x | ALoc x => (var_expr (name_var x), [ {| fact_R:=str_rel x; fact_args:=[in_timestamp; var_expr (name_var x)] |} ])
+        | AVar x => (var_expr (singleton_var x), [])
+        | ALoc x => (var_expr (singleton_var x), [ {| fact_R:=str_rel x; fact_args:=[in_timestamp; var_expr (singleton_var x)] |} ])
         | ABool b => (fun_expr (fnB (fn_BLit b)) [], [])
         | AInt n => (fun_expr (fnZ (fn_ZLit n)) [], [])
         | AString s => (fun_expr (fnS (fn_SLit s)) [], [])
-        | ALet e1 x e2 => let '(e1', conds1) := lower_aexpr m e1 in
-                          let '(e2', conds2) := lower_aexpr m e2 in
-                          (e2', {| fact_R:=str_rel x; fact_args:=[in_timestamp; e1'] |} :: conds1 ++ conds2)
-        | ANot e => let '(e', conds) := lower_aexpr m e in
+        | ALet e1 x e2 => let '(e1', conds1) := lower_aexpr e1 in
+                          let '(e2', conds2) := lower_aexpr e2 in
+                          (e2', {| fact_R:=true_rel; fact_args:=[fun_expr (fnB fn_Eq) [var_expr (singleton_var x); e1']] |} :: conds1 ++ conds2)
+        | ANot e => let '(e', conds) := lower_aexpr e in
                     (fun_expr (fnB fn_Not) [e'], conds)
-        | AAnd e1 e2 => let '(e1', conds1) := lower_aexpr m e1 in
-                        let '(e2', conds2) := lower_aexpr m e2 in
+        | AAnd e1 e2 => let '(e1', conds1) := lower_aexpr e1 in
+                        let '(e2', conds2) := lower_aexpr e2 in
                         (fun_expr (fnB fn_And) [e1'; e2'], conds1 ++ conds2)
-        | APlus e1 e2 => let '(e1', conds1) := lower_aexpr m e1 in
-                         let '(e2', conds2) := lower_aexpr m e2 in
+        | APlus e1 e2 => let '(e1', conds1) := lower_aexpr e1 in
+                         let '(e2', conds2) := lower_aexpr e2 in
                          (fun_expr (fnZ fn_Plus) [e1'; e2'], conds1 ++ conds2)
-        | AStringConcat e1 e2 => let '(e1', conds1) := lower_aexpr m e1 in
-                                 let '(e2', conds2) := lower_aexpr m e2 in
+        | AStringConcat e1 e2 => let '(e1', conds1) := lower_aexpr e1 in
+                                 let '(e2', conds2) := lower_aexpr e2 in
                                  (fun_expr (fnS fn_StringConcat) [e1'; e2'], conds1 ++ conds2)
-        | AStringLength e => let '(e', conds) := lower_aexpr m e in
+        | AStringLength e => let '(e', conds) := lower_aexpr e in
                              (fun_expr (fnZ fn_StringLength) [e'], conds)
-        | AAccess x attr => (match map.get m (x, attr) with
-                             | Some x' => var_expr x'
-                             | None => fun_expr (fnB (fn_BLit false)) [] (* unreachable *)
-                             end, [])
+        | AAccess x attr => (var_expr (access_var (x, attr)), [])
         end.
 
-      Definition lower_pexpr (m : attrenv) (e : pexpr) : (dexpr * list fact) :=
+      Definition lower_pexpr (e : pexpr) : (dexpr * list fact) :=
         match e with
         | PLt e1 e2 =>
-            let '(e1', conds1) := lower_aexpr m e1 in
-            let '(e2', conds2) := lower_aexpr m e2 in
+            let '(e1', conds1) := lower_aexpr e1 in
+            let '(e2', conds2) := lower_aexpr e2 in
             (fun_expr (fnB fn_Lt) [e1'; e2'], conds1 ++ conds2)
         | PEq e1 e2 =>
-            let '(e1', conds1) := lower_aexpr m e1 in
-            let '(e2', conds2) := lower_aexpr m e2 in
+            let '(e1', conds1) := lower_aexpr e1 in
+            let '(e2', conds2) := lower_aexpr e2 in
             (fun_expr (fnB fn_Eq) [e1'; e2'], conds1 ++ conds2)
         end.
 
@@ -212,54 +213,100 @@ Section __.
                             end
         end.
 
-      Definition lower_rexpr (Gstore Genv : tenv) (m : attrenv) (e : rexpr) : list dexpr * list fact * list (string * type) :=
+      Definition get_rexpr_type (Gstore Genv : tenv) (r : rexpr) : type :=
+        match r with
+          RRecord l =>
+            TRecord
+              (List.map (fun '(attr, a) => (attr, get_aexpr_type Gstore Genv a)) l)
+        end.
+
+      Fixpoint get_expr_type (Gstore : tenv) (e : expr) : type :=
+        match e with
+        | EAtom a => get_aexpr_type Gstore map.empty a
+        | ELoc x => match map.get Gstore x with
+                    | Some t => t
+                    | _ => TBool (* unused case *)
+                    end
+        | EEmptySet tl => TSet (TRecord tl)
+        | ESetInsert r e => get_expr_type Gstore e
+        | EFilter e x p => get_expr_type Gstore e
+        | EJoin e1 e2 x1 x2 p r =>
+            match get_expr_type Gstore e1 with
+            | TSet t1 =>
+                match get_expr_type Gstore e2 with
+                | TSet t2 =>
+                    TSet (get_rexpr_type Gstore (map.put (map.put map.empty x1 t1) x2 t2) r)
+                | _ => TBool
+                end
+            | _ => TBool
+            end
+        | EProj e x r =>
+            match get_expr_type Gstore e with
+            | TSet t =>
+                TSet (get_rexpr_type Gstore (map.put map.empty x t) r)
+            | _ => TBool
+            end
+        end.
+
+
+      Definition lower_rexpr (Gstore Genv : tenv) (e : rexpr) : list dexpr * list fact * list (string * dtype) :=
         match e with
           RRecord l =>
-            (List.map (fun '(_, a) => fst (lower_aexpr m a)) (record_sort l),
-              List.concat (List.map (fun '(_, a) => snd (lower_aexpr m a)) (record_sort l)),
-              List.map (fun '(s, a) => (s, get_aexpr_type Gstore Genv a)) (record_sort l))
+            (List.map (fun '(_, a) => fst (lower_aexpr a)) (record_sort l),
+              List.concat (List.map (fun '(_, a) => snd (lower_aexpr a)) (record_sort l)),
+              List.map (fun '(s, a) => (s, lower_type (get_aexpr_type Gstore Genv a))) (record_sort l))
         end.
 
-      Fixpoint mk_vars (name : string) (tl : list (string * type)) : list var :=
-        match tl with
+      Fixpoint mk_vars (name : string) (attrs : list string) : list var :=
+        match attrs with
         | [] => []
-        | (attr, _) :: tl => attr_var (name, attr) :: (mk_vars name tl)
+        | attr :: attrs => access_var (name, attr) :: (mk_vars name attrs)
         end.
 
+      (* ??? remove
       Fixpoint put_attr_bindings (m : attrenv) (x : string) (attrs : list string) (vars : list var) : attrenv :=
         match attrs, vars with
         | [], _ | _, [] => m
         | attr :: attrs, v :: vars =>
             map.put (put_attr_bindings m x attrs vars) (x, attr) v
         end.
-
+*)
       Definition lower_rec_type : list (string * type) -> list (string * dtype) :=
         List.map (fun '(s, t) => (s, lower_type t)).
     End WithTimestamp.
+
+    Definition dexpr_zero : dexpr := fun_expr (fnZ (fn_ZLit 0)) [].
+    Definition dexpr_plus_one (e : dexpr) :=
+      fun_expr (fnZ fn_Plus) [e; fun_expr (fnZ (fn_ZLit 1)) []].
 
     Section WithTimestamp.
       Section WithGstore.
         Context (Gstore : tenv).
         Context (blk_hyps : list fact). (* assumptions created in lower_block *)
 
-        Fixpoint lower_expr (in_timestamp out_timestamp : dexpr) (out : rel) (next_rel : nat) (e : expr) :
-          list decl * list rule * nat * list (string * type) :=
+        Fixpoint lower_expr (to_next_ts : bool) (out : rel) (next_rel : nat) (e : expr) :
+          list decl * list rule * nat * list (string * dtype) :=
+          let in_timestamp := var_expr time_var in
+          let out_timestamp := if to_next_ts
+                               then dexpr_plus_one in_timestamp
+                               else in_timestamp in
           match e with
           | EAtom a =>
-              let '(a', asms) := lower_aexpr in_timestamp map.empty a in
+              let '(a', asms) := lower_aexpr in_timestamp a in
               ([],
                 [{| rule_concls := [{| fact_R := out; fact_args := [out_timestamp; a'] |}];
                    rule_hyps := asms ++ blk_hyps;
                    rule_agg := None;
                    rule_set_hyps := [] |}],
                 next_rel,
-                [(singleton_attr, get_aexpr_type Gstore map.empty a)])
+                [(singleton_attr, lower_type (get_aexpr_type Gstore map.empty a))])
           | ELoc x =>
-              let attr_tys := match map.get Gstore x with
-                              | Some (TSet (TRecord l)) => l
+              let tl := match map.get Gstore x with
+                              | Some (TSet (TRecord tl)) => tl
                               | _ => [] (* unreachable for well-typed expressions *)
                               end in
-              let vs := List.map var_expr (mk_vars x attr_tys) in
+              let attr_tys := lower_rec_type tl in
+              let vs := List.map (fun x => var_expr (attr_var x)) (List.map fst tl) in
               ([],
                 [{| rule_concls := [{| fact_R := out; fact_args := out_timestamp :: vs |}];
                    rule_hyps := [{| fact_R := str_rel x; fact_args := in_timestamp :: vs|}] ++ blk_hyps;
@@ -267,14 +314,18 @@ Section __.
                    rule_set_hyps := [] |}],
                 next_rel,
                 attr_tys)
-          | EEmptySet tl => ([], [], next_rel, tl)
+          | EEmptySet tl => ([], [], next_rel, lower_rec_type tl)
           | ESetInsert r s =>
-              let '(r', asms, _) := lower_rexpr in_timestamp Gstore map.empty map.empty r in
+              let '(r', asms, _) := lower_rexpr in_timestamp Gstore map.empty r in
               let aux := nat_rel next_rel in
-              let '(dcls, rls, next_rel', attr_tys) := lower_expr in_timestamp in_timestamp aux (S next_rel) s in
-              let vs := List.map var_expr (mk_vars "" attr_tys) in
+              let '(dcls, rls, next_rel', attr_tys) := lower_expr false aux (S next_rel) s in
+              let tl := match get_rexpr_type Gstore map.empty r with
+                        | TSet (TRecord tl) => tl
+                        | _ => []
+                        end in
+              let vs := List.map (fun attr => var_expr (attr_var attr)) (List.map fst tl) in
               (dcls ++
-                 [ {| decl_R := aux; decl_sig := lower_rec_type ((timestamp_attr, TInt) :: attr_tys) |} ],
+                 [ {| decl_R := aux; decl_sig := (timestamp_attr, DNumber) :: attr_tys |} ],
                 rls ++
                   [ {| rule_concls := [{| fact_R := out; fact_args := out_timestamp :: r' |}];
                       rule_hyps := asms ++ blk_hyps;
@@ -289,14 +340,18 @@ Section __.
           | EFilter s x p =>
               (* out vs :- aux vs, p *)
               let aux := nat_rel next_rel in
-              let '(dcls, rls, next_rel', attr_tys) := lower_expr in_timestamp in_timestamp aux (S next_rel) s in
-              let vars := mk_vars x attr_tys in
-              let p_asms := List.map (lower_pexpr in_timestamp (put_attr_bindings map.empty x (List.map fst attr_tys) vars)) p in
+              let '(dcls, rls, next_rel', attr_tys) := lower_expr false aux (S next_rel) s in
+              let tl := match get_expr_type Gstore s with
+                        | TSet (TRecord tl) => tl
+                        | _ => []
+                        end in
+              let vars := mk_vars x (List.map fst tl) in
+              let p_asms := List.map (lower_pexpr in_timestamp) p in
               let ps' := List.map fst p_asms in
               let asms := List.concat (List.map snd p_asms) in
               let vs := List.map var_expr vars in
               (dcls ++
-                 [ {| decl_R := aux; decl_sig := lower_rec_type ((timestamp_attr, TInt) :: attr_tys) |} ],
+                 [ {| decl_R := aux; decl_sig := (timestamp_attr, DNumber) :: attr_tys |} ],
                 rls ++
                   [ {| rule_concls := [ {| fact_R := out; fact_args := out_timestamp :: vs |} ];
                       rule_hyps := [ {| fact_R := aux; fact_args := in_timestamp :: vs |} ] ++
@@ -307,23 +362,31 @@ Section __.
                 next_rel',
                 attr_tys)
           | EJoin s1 s2 x1 x2 p r =>
-              (* out (lower_rexpr m r) :- aux1 vs1, aux2 vs2, lower_aexpr m p *)
+              (* out (lower_rexpr m r) :- aux1 vs1, aux2 vs2, lower_aexpr p *)
               let aux1 := nat_rel next_rel in
-              let '(dcls1, rls1, next_rel1, attr_tys1) := lower_expr in_timestamp in_timestamp aux1 (S next_rel) s1 in
+              let '(dcls1, rls1, next_rel1, attr_tys1) := lower_expr false aux1 (S next_rel) s1 in
               let aux2 := nat_rel next_rel1 in
-              let '(dcls2, rls2, next_rel2, attr_tys2) := lower_expr in_timestamp in_timestamp aux2 (S next_rel1) s2 in
-              let vars1 := mk_vars x1 attr_tys1 in
-              let vars2 := mk_vars x2 attr_tys2 in
-              let m := put_attr_bindings (put_attr_bindings map.empty x1 (List.map fst attr_tys1) vars1) x2 (List.map fst attr_tys2) vars2 in
+              let '(dcls2, rls2, next_rel2, attr_tys2) := lower_expr false aux2 (S next_rel1) s2 in
+              let tl1 := match get_expr_type Gstore s1 with
+                         | TSet (TRecord tl1) => tl1
+                         | _ => []
+                         end in
+              let tl2 := match get_expr_type Gstore s2 with
+                         | TSet (TRecord tl2) => tl2
+                         | _ => []
+                         end in
+              let vars1 := mk_vars x1 (List.map fst tl1) in
+              let vars2 := mk_vars x2 (List.map fst tl2) in
               let vs1 := List.map var_expr vars1 in
               let vs2 := List.map var_expr vars2 in
-              let p_asms := List.map (lower_pexpr in_timestamp m) p in
+              let p_asms := List.map (lower_pexpr in_timestamp) p in
               let ps' := List.map fst p_asms in
               let asms_p := List.concat (List.map snd p_asms) in
-              let '(r', asms_r, attr_tys) := lower_rexpr in_timestamp Gstore (map.put (map.put map.empty x1 (TRecord attr_tys1)) x2 (TRecord attr_tys2)) m r in
+              let Genv := map.put (map.put map.empty x1 (TRecord tl1)) x2 (TRecord tl2) in
+              let '(r', asms_r, attr_tys) := lower_rexpr in_timestamp Gstore Genv r in
               (dcls1 ++ dcls2 ++
-                 [ {| decl_R := aux1; decl_sig := lower_rec_type ((timestamp_attr, TInt) :: attr_tys1) |};
-                   {| decl_R := aux2; decl_sig := lower_rec_type ((timestamp_attr, TInt) :: attr_tys2) |} ],
+                 [ {| decl_R := aux1; decl_sig := (timestamp_attr, DNumber) :: attr_tys1 |};
+                   {| decl_R := aux2; decl_sig := (timestamp_attr, DNumber) :: attr_tys2 |} ],
                 rls1 ++ rls2 ++
                   [ {| rule_concls := [ {| fact_R := out; fact_args := out_timestamp :: r' |} ] ;
                       rule_hyps :=
@@ -338,12 +401,17 @@ Section __.
           | EProj s x r =>
               (* out rs :- aux vs *)
               let aux := nat_rel next_rel in
-              let '(dcls, rls, next_rel', attr_tys) := lower_expr in_timestamp in_timestamp aux (S next_rel) s in
-              let vars := mk_vars x attr_tys in
-              let '(r', asms, out_attr_tys) := lower_rexpr in_timestamp Gstore (map.put map.empty x (TRecord attr_tys)) (put_attr_bindings map.empty x (List.map fst attr_tys) vars) r in
+              let '(dcls, rls, next_rel', attr_tys) := lower_expr false aux (S next_rel) s in
+              let tl := match get_expr_type Gstore s with
+                        | TSet (TRecord tl) => tl
+                        | _ => []
+                        end in
+              let vars := mk_vars x (List.map fst attr_tys) in
+              let Genv := map.put map.empty x (TRecord tl) in
+              let '(r', asms, out_attr_tys) := lower_rexpr in_timestamp Gstore Genv r in
               let vs := List.map var_expr vars in
               (dcls ++
-                 [ {| decl_R := aux; decl_sig := lower_rec_type ((timestamp_attr, TInt) :: attr_tys) |} ],
+                 [ {| decl_R := aux; decl_sig := (timestamp_attr, DNumber) :: attr_tys |} ],
                 rls ++
                   [ {| rule_concls := [ {| fact_R := out; fact_args := out_timestamp :: r' |} ];
                       rule_hyps := [ {| fact_R := aux; fact_args := in_timestamp :: vs |} ] ++ asms ++ blk_hyps;
@@ -361,102 +429,498 @@ Section __.
       | (x, t) :: muts => map.put (mk_tenv muts) x t
       end.
 
-    Definition dexpr_plus_one (e : dexpr) :=
-      fun_expr (fnZ fn_Plus) [e; fun_expr (fnZ (fn_ZLit 1)) []].
-
-    Fixpoint lower_mut_assignments (hyps : list fact) (Gstore : tenv) (next_rel : nat) (asgs : list (string * expr)) : list decl * list rule * nat :=
+    (* ??? remove
+    Fixpoint lower_mut_assignments0 (next_rel : nat) (asgs : list (string * expr)) :
+      list decl * list rule * nat :=
+      match asgs with
+      | [] => ([], [], next_rel)
+      | (x, e) :: asgs =>
+          let '(dcls0, rls0, next_rel0, _) :=
+            lower_expr map.empty
+              [] (* no hypothesis at entry *)
+              dexpr_zero (* out_timestamp*)
+              dexpr_zero (* in_timestamp *)
+              (str_rel x) next_rel e in
+          let '(dcls, rls, next_rel') :=
+            lower_mut_assignments0 next_rel0 asgs in
+          (dcls0 ++ dcls, rls0 ++ rls, next_rel')
+      end.
+*)
+    Fixpoint lower_mut_assignments (hyps : list fact) (Gstore : tenv) (next_rel : nat) (asgs : list (string * expr)) :
+          list decl * list rule * nat :=
       match asgs with
       | [] => ([], [], next_rel)
       | (x, e) :: asgs =>
           let '(dcls0, rls0, next_rel0, _) :=
             lower_expr Gstore
             hyps (* blk_hyps *)
-            (dexpr_plus_one (var_expr time_var)) (* out_timestamp*)
-            (var_expr time_var) (* in_timestamp *)
+            true (* increment timestamp *)
             (str_rel x) next_rel e in
           let '(dcls, rls, next_rel') :=
             lower_mut_assignments hyps Gstore next_rel0 asgs in
           (dcls0 ++ dcls, rls0 ++ rls, next_rel')
       end.
 
-    Definition lower_block (g : cfg) (next_rel : nat) (blk_id : nat) : list decl * list rule * nat :=
-      let '(muts, blks) := g in
-      let Gstore := mk_tenv muts in
-      match nth_error blks blk_id with
-      | Some blk =>
-          match blk with
-          | BGoto (n, es) =>
-              let '(dcls, rls, next_rel') :=
-                lower_mut_assignments
-                  [{| fact_R := blk_rel blk_id; fact_args := [var_expr time_var] |}]
-                  Gstore next_rel (combine (List.map fst muts) es) in
-              (dcls,
-                rls ++
-                  [{| rule_concls := [ {| fact_R := blk_rel n; fact_args := [dexpr_plus_one (var_expr time_var)] |} ];
-                     rule_hyps := [ {| fact_R := blk_rel blk_id; fact_args := [var_expr time_var]|} ];
-                     rule_agg := None;
-                     rule_set_hyps := [] |}], next_rel')
-          | BIf p (n1, es1) (n2, es2) =>
-              let '(p', asms) := lower_pexpr (var_expr time_var) map.empty p in
-              let '(dcls1, rls1, next_rel1) :=
-                lower_mut_assignments
-                  ([{| fact_R := blk_rel blk_id; fact_args := [var_expr time_var] |};
-                   {| fact_R := true_rel; fact_args := [p'] |} ] ++ asms)
-                  Gstore next_rel (combine (List.map fst muts) es1) in
-              let neg_p' := fun_expr (fnB fn_Not) [p'] in
-              let '(dcls2, rls2, next_rel2) :=
-                lower_mut_assignments
-                  ([{| fact_R := blk_rel blk_id; fact_args := [var_expr time_var] |};
-                   {| fact_R := true_rel; fact_args := [neg_p'] |} ] ++ asms)
-                  Gstore next_rel (combine (List.map fst muts) es2) in
-              (dcls1 ++ dcls2,
-                rls1 ++ rls2 ++
-                  [{| rule_concls := [{| fact_R := blk_rel n1; fact_args := [dexpr_plus_one (var_expr time_var)] |}];
-                     rule_hyps := [{| fact_R := blk_rel blk_id; fact_args := [var_expr time_var] |};
-                                   {| fact_R := true_rel; fact_args := [p'] |} ] ++ asms;
-                     rule_agg := None;
-                     rule_set_hyps := [] |};
-                  {| rule_concls := [{| fact_R := blk_rel n2; fact_args := [dexpr_plus_one (var_expr time_var)] |}];
-                     rule_hyps := [{| fact_R := blk_rel blk_id; fact_args := [var_expr time_var] |};
-                                   {| fact_R := true_rel; fact_args := [neg_p'] |} ] ++ asms;
-                     rule_agg := None;
-                     rule_set_hyps := [] |}],
-              next_rel2)
-
-          | BRet =>
-              ([],
-                [ {| rule_concls := [ {| fact_R := ret_rel ; fact_args := [var_expr time_var] |} ];
-                    rule_hyps := [ {| fact_R := blk_rel blk_id; fact_args := [var_expr time_var] |} ];
-                    rule_agg := None;
-                    rule_set_hyps := [] |} ], next_rel)
-          end
-      | None => ([], [], 0) (* unreachable case *)
+    Definition lower_block (sig : list (string * type)) (next_rel : nat) (blk : block) (blk_id : nat) :
+      list decl * list rule * nat :=
+      let Gstore := mk_tenv sig in
+      match blk with
+      | BGoto es n =>
+          let '(dcls, rls, next_rel') :=
+            lower_mut_assignments
+              [{| fact_R := blk_rel blk_id; fact_args := [var_expr time_var] |}]
+              Gstore next_rel (combine (List.map fst sig) es) in
+          (dcls,
+            rls ++
+              [{| rule_concls := [ {| fact_R := blk_rel n; fact_args := [dexpr_plus_one (var_expr time_var)] |} ];
+                 rule_hyps := [ {| fact_R := blk_rel blk_id; fact_args := [var_expr time_var]|} ];
+                 rule_agg := None;
+                 rule_set_hyps := [] |}], next_rel')
+      | BIf p es1 n1 es2 n2 =>
+          let '(p', asms) := lower_pexpr (var_expr time_var) p in
+          let '(dcls1, rls1, next_rel1) :=
+            lower_mut_assignments
+              ([{| fact_R := blk_rel blk_id; fact_args := [var_expr time_var] |};
+                {| fact_R := true_rel; fact_args := [p'] |} ] ++ asms)
+              Gstore next_rel (combine (List.map fst sig) es1) in
+          let neg_p' := fun_expr (fnB fn_Not) [p'] in
+          let '(dcls2, rls2, next_rel2) :=
+            lower_mut_assignments
+              ([{| fact_R := blk_rel blk_id; fact_args := [var_expr time_var] |};
+                {| fact_R := true_rel; fact_args := [neg_p'] |} ] ++ asms)
+              Gstore next_rel (combine (List.map fst sig) es2) in
+          (dcls1 ++ dcls2,
+            rls1 ++ rls2 ++
+              [{| rule_concls := [{| fact_R := blk_rel n1; fact_args := [dexpr_plus_one (var_expr time_var)] |}];
+                 rule_hyps := [{| fact_R := blk_rel blk_id; fact_args := [var_expr time_var] |};
+                               {| fact_R := true_rel; fact_args := [p'] |} ] ++ asms;
+                 rule_agg := None;
+                 rule_set_hyps := [] |};
+               {| rule_concls := [{| fact_R := blk_rel n2; fact_args := [dexpr_plus_one (var_expr time_var)] |}];
+                 rule_hyps := [{| fact_R := blk_rel blk_id; fact_args := [var_expr time_var] |};
+                               {| fact_R := true_rel; fact_args := [neg_p'] |} ] ++ asms;
+                 rule_agg := None;
+                 rule_set_hyps := [] |}],
+            next_rel2)
+      | BRet =>
+          ([],
+            [ {| rule_concls := [ {| fact_R := ret_rel ; fact_args := [var_expr time_var] |} ];
+                rule_hyps := [ {| fact_R := blk_rel blk_id; fact_args := [var_expr time_var] |} ];
+                rule_agg := None;
+                rule_set_hyps := [] |} ], next_rel)
       end.
 
-    Fixpoint lower_blocks (g : cfg) (next_rel : nat) (blk_id : nat) : list decl * list rule * nat :=
-      match blk_id with
-      | O => lower_block g next_rel O
-      | S n => let '(dcls1, rls1, next_rel1) := lower_blocks g next_rel n in
-               let '(dcls2, rls2, next_rel2) := lower_block g next_rel1 (S n) in
-               (dcls1 ++ dcls2, rls1 ++ rls2, next_rel2)
+    Fixpoint lower_blocks  (sig : list (string * type)) (next_rel : nat) (blks : list block) (cur_id : nat) : list decl * list rule * nat :=
+      match blks with
+      | [] => ([], [], next_rel)
+      | blk :: blks =>
+          let '(dcls1, rls1, next_rel1) := lower_block sig next_rel blk cur_id in
+          let '(dcls2, rls2, next_rel2) := lower_blocks sig next_rel1 blks (S cur_id) in
+          (dcls1 ++ dcls2, rls1 ++ rls2, next_rel2)
+      end.
+
+    Definition lower_mut_res (mut_ty : (string * type)) : rule :=
+      let '(x, t) := mut_ty in
+      match t with
+      | TSet (TRecord tl)
+      | TRecord tl =>
+          let vs := List.map (fun x => var_expr (attr_var x)) (List.map fst tl) in
+          {| rule_concls := [ {| fact_R := res_rel x; fact_args := vs |} ];
+            rule_hyps := [ {| fact_R := ret_rel; fact_args := [var_expr time_var] |};
+                           {| fact_R := str_rel x; fact_args := var_expr time_var :: vs |}];
+            rule_agg := None;
+            rule_set_hyps := [] |}
+      | t =>
+          let v := var_expr (singleton_var x) in
+          {| rule_concls := [ {| fact_R := res_rel x; fact_args := [v] |} ];
+            rule_hyps := [ {| fact_R := ret_rel; fact_args := [var_expr time_var] |};
+                           {| fact_R := str_rel x; fact_args := [var_expr time_var; v] |}];
+            rule_agg := None;
+            rule_set_hyps := [] |}
+      end.
+
+    Definition decl_mut_rels (p : string *  type) : list decl :=
+      let '(x, t) := p in
+      match t with
+      | TSet (TRecord tl)
+      | TRecord tl =>
+          [ {| decl_R := str_rel x;
+              decl_sig := (timestamp_attr, DNumber) :: lower_rec_type tl |};
+            {| decl_R := res_rel x;
+              decl_sig := lower_rec_type tl |} ]
+      | _ =>
+          [ {| decl_R := str_rel x;
+              decl_sig := (timestamp_attr, DNumber) :: [(singleton_attr, lower_type t)] |};
+            {| decl_R := res_rel x;
+              decl_sig := [(singleton_attr, lower_type t)] |} ]
+      end.
+
+    Definition lower_atomic_value (v : value) : obj :=
+      match v with
+      | VInt n => Zobj n
+      | VBool b => Bobj b
+      | VString s => Sobj s
+      (* unused cases *)
+      | VList _ | VRecord _ | VSet _ => Bobj false
+      end.
+
+    Definition lower_rec_value (v : value) : list obj :=
+      match v with
+      | VRecord l => map (fun p => lower_atomic_value (snd p)) l
+      | _ => []
+      end.
+
+    Definition dexpr_literal (v : obj) : dexpr :=
+      match v with
+      | Bobj b => fun_expr (fnB (fn_BLit b)) []
+      | Zobj z => fun_expr (fnZ (fn_ZLit z)) []
+      | Sobj s => fun_expr (fnS (fn_SLit s)) []
+      end.
+
+    Definition lower_init_value (out : rel) (v : value) : list rule :=
+      match v with
+      | VSet l => map (fun v =>
+                         {| rule_concls :=
+                             [ {| fact_R := out;
+                                 fact_args := dexpr_zero :: map dexpr_literal (lower_rec_value v) |} ];
+                           rule_hyps := [];
+                           rule_agg := None;
+                           rule_set_hyps := [] |}) l
+      | VRecord _ => [ {| rule_concls :=
+                             [ {| fact_R := out;
+                                 fact_args := dexpr_zero :: map dexpr_literal (lower_rec_value v) |} ];
+                           rule_hyps := [];
+                           rule_agg := None;
+                           rule_set_hyps := [] |} ]
+      | v => [ {| rule_concls :=
+                   [ {| fact_R := out;
+                       fact_args := [ dexpr_zero; dexpr_literal (lower_atomic_value v) ] |} ];
+                       rule_hyps := [];
+                       rule_agg := None;
+                       rule_set_hyps := [] |} ]
       end.
 
     Definition lower_cfg (g : cfg) : list decl * list rule :=
-      let '(muts_tys, blks) := g in
-      let mut_dcls := List.map
-                        (fun '(x, t) =>
-                           {| decl_R := str_rel x;
-                             decl_sig := match t with
-                                         | TSet (TRecord tl) => (timestamp_attr, DNumber) :: lower_rec_type tl
-                                         | t => [(timestamp_attr, DNumber); (singleton_attr, lower_type t)]
-                                         end |})
-                        muts_tys in
-      let '(dcls, rls, _) := match List.length blks with
-                             | O => ([], [], 0)
-                             | S n => lower_blocks g O n
-                             end in
-      (mut_dcls ++ dcls, rls).
+      let g_sig := g.(sig_blks).(sig) in
+      let mut_dcls := List.concat (map decl_mut_rels g_sig) in
+      let init_str_rls := List.concat
+                            (map (fun '(x, v) => lower_init_value (str_rel x) v)
+                               (combine (map fst g_sig) g.(str_ptr).(str))) in
+      let entry_blk_rl :=
+        match g.(str_ptr).(ptr) with
+        | Some n =>
+            {| rule_concls :=
+                [{| fact_R := blk_rel n; fact_args := [dexpr_zero] |}];
+              rule_hyps := [];
+              rule_agg := None;
+              rule_set_hyps := [] |}
+        | None =>
+            {| rule_concls :=
+                [{| fact_R := ret_rel; fact_args := [dexpr_zero] |}];
+              rule_hyps := [];
+              rule_agg := None;
+              rule_set_hyps := [] |}
+        end in
+      let '(dcls, rls, _) := lower_blocks g_sig O g.(sig_blks).(blks) O in
+      let res_rls := List.map lower_mut_res g_sig in
+      (mut_dcls ++ dcls,
+        entry_blk_rl ::
+          init_str_rls ++ rls ++ res_rls).
+
+    Context {venv: map.map string value} {venv_ok: map.ok venv}.
+    Context {context : map.map var obj} {context_ok: map.ok context}.
+
+    Definition lower_value (v : value) : list (list obj) :=
+      (* lower source language value to set of datalog obj tuples *)
+      match v with
+      | VSet l => map lower_rec_value l
+      | VRecord _ => [ lower_rec_value v ]
+      | v => (* atomic value *)
+          [ [ lower_atomic_value v ] ]
+      end.
+
+    Definition is_lowered_to_at (v : value) (rls : list rule) (res : rel) (ts : Z) : Prop :=
+      Forall (fun vs => prog_impl_fact rls (res, Zobj ts :: vs)) (lower_value v).
+
+    Definition is_lowered_from_at (rls : list rule) (res : rel) (v : value) (ts : Z) : Prop :=
+      forall vs', prog_impl_fact rls (res, Zobj ts :: vs') ->
+                  In vs' (lower_value v).
+
+    Definition is_lowered_to (v : value) (rls : list rule) (res : rel) : Prop :=
+      Forall (fun vs => prog_impl_fact rls (res, vs)) (lower_value v).
+
+    Definition is_lowered_from (rls : list rule) (res : rel) (v : value) : Prop :=
+      forall vs', prog_impl_fact rls (res, vs') ->
+                  In vs' (lower_value v).
+
+    Definition venv_is_lowered_to_at (muts : list string) (str : list value) (rls : list rule) (ts : Z) : Prop :=
+      Forall2 (fun x v => is_lowered_to_at v rls (str_rel x) ts) muts str.
+
+    Definition venv_is_lowered_to (muts : list string) (str : list value) (rls : list rule) : Prop :=
+      Forall2 (fun x v => is_lowered_to v rls (res_rel x)) muts str.
+
+    Definition venv_is_lowered_from_at (rls : list rule) (muts : list string) (str : list value) (ts : Z) : Prop :=
+      Forall2 (fun x v => is_lowered_from_at rls (res_rel x) v ts) muts str.
+
+    Definition venv_is_lowered_from (rls : list rule) (muts : list string) (str : list value) : Prop :=
+      Forall2 (fun x v => is_lowered_from rls (res_rel x) v) muts str.
+
+    (* ???
+    Lemma lower_cfg_complete'' : forall (g : cfg) (store : venv) dcls rls n ts store' m,
+        lower_cfg g = (dcls, rls) ->
+        well_typed_block g.(sig) g.(blks) n ->
+        block_step g.(sig) g.(blks) store n store' m ->
+        venv_is_lowered_to_at Gstore store rls ts ->
+        prog_impl_fact rls (blk_rel n, [Zobj (Z.of_nat ts)]) ->
+        match m with
+        | Some n' =>
+            venv_is_lowered_to_at Gstore store' rls (S ts) /\
+              prog_impl_fact rls (blk_rel n, [Zobj (Z.of_nat ts + 1)])
+        | None => store' = store /\
+                    venv_is_lowered_to Gstore store' rls
+        end.
+      Admitted.
+
+    Lemma lower_cfg_complete' : forall (g : cfg) (Gstore : tenv) (store : venv) dcls rls n ts store' m,
+        lower_cfg g = (dcls, rls) ->
+        Gstore = mk_tenv g.(sig) ->
+        well_typed_cfg g ->
+        block_steps g.(sig) g.(blks) store n store' m ->
+        venv_is_lowered_to_at Gstore store rls ts ->
+        prog_impl_fact rls (blk_rel n, [Zobj (Z.of_nat ts)]) ->
+        match m with
+        | Some n' =>
+            exists ts',
+            venv_is_lowered_to_at Gstore store' rls ts' /\
+              prog_impl_fact rls (blk_rel n, [Zobj (Z.of_nat ts')])
+        | None => venv_is_lowered_to Gstore store' rls
+        end.
+    Admitted.
+     *)(*
+
+    Lemma lower_cfg_complete'' : forall (g : cfg) (store : venv) dcls rls blk n ts store' m,
+        lower_cfg g = (dcls, rls) ->
+        (* well_typed_block g.(sig) (List.length g.(blks)) blk -> *)
+        venv_is_lowered_to_at (mk_tenv g.(sig)) store rls ts ->
+        nth_error g.(blks) n = Some blk ->
+        prog_impl_fact rls (blk_rel n, [Zobj ts]) ->
+        block_step g.(sig) store blk store' m ->
+        match m with
+        | Some n' =>
+            venv_is_lowered_to_at (mk_tenv g.(sig)) store' rls (ts + 1) /\
+              prog_impl_fact rls (blk_rel n', [Zobj (ts + 1)])
+        | None => store' = store /\
+                    venv_is_lowered_to (mk_tenv g.(sig)) store' rls
+        end.
+    Proof.
+      intros. inversion H3; subst.
+      1:{ unfold lower_cfg in *.
+    Admitted.
+
+    Lemma lower_mut_assignments_complete : forall hyps Gstore sig0 args next_rel dcls rls next_rel',
+        Forall2 (fun (e : expr) (t : type) => type_of_expr Gstore e t)
+          args (map snd sig0) ->
+        lower_mut_assignments hyps Gstore next_rel (combine (map fst sig0) args) = (dcls, rls, next_rel') ->
+        venv_is_lowered_to_at (mk_tenv sig0)
+          (mk_venv (map fst sig0) (map (interp_expr map.empty) args))
+          rls 0.
+
+    Lemma lower_expr_complete : forall Gstore store blk_hyps in_ts out_ts out next_rel e dcls rls rls0 next_rel' tl' in_v out_v ctx t,
+        lower_expr Gstore blk_hyps in_ts out_ts out next_rel e =
+          (dcls, rls, next_rel', tl') ->
+        type_of_expr Gstore e t ->
+        incl rls rls0 ->
+        (forall (x,t) in Gstore, (x,v) in store,
+           prog_impl_fact rls0 (str_rel x, [in_v; x_v])) ->
+      (forall h, In h hyps,
+      interp_fact ctx? h h' ->
+      prog_impl_fact rls0 h') ->
+
+        Datalog.interp_expr ctx? in_ts (Zobj in_v) ->
+        Datalog.interp_expr ctx? out_ts (Zobj out_v) ->
+        tenv_wf Gstore ->
+        venv_wf Gstore store ->
+        is_lowered_to_at t (interp_expr store e) rls out out_v.
+
+    Lemma lower_mut_assignments0_complete : forall sig0 args next_rel dcls rls next_rel',
+        Forall2 (fun (e : expr) (t : type) => type_of_expr map.empty e t)
+          args (map snd sig0) ->
+        lower_mut_assignments0 next_rel (combine (map fst sig0) args) = (dcls, rls, next_rel') ->
+        venv_is_lowered_to_at (mk_tenv sig0)
+          (mk_venv (map fst sig0) (map (interp_expr map.empty) args))
+          rls 0.
+    Proof.
+      intros *. remember (map snd sig0) as l.
+      induction 1; destruct sig0; try discriminate; cbn in *.
+        *)
+
+    Lemma prog_impl_fact_weaken : forall (rls rls' : list rule) f,
+      prog_impl_fact rls f -> incl rls rls' ->
+      prog_impl_fact rls' f.
+    Proof.
+      unfold prog_impl_fact.
+      induction 1. intros.
+      econstructor.
+      1: eapply incl_Exists; eauto.
+      rewrite Forall_forall; intros.
+      apply_Forall_In.
+    Qed.
+
+    Ltac invert_type_of_value :=
+      lazymatch goal with
+        H: type_of_value _ _ |- _ =>
+          inversion H; subst; clear H
+      end.
+
+    Ltac invert_SSorted :=
+      lazymatch goal with
+        H: Sorted.StronglySorted _ (_ :: _) |- _ =>
+          inversion H; subst
+      end.
+
+    Lemma interp_expr__dexpr_literal_atomic : forall vl tl,
+        type_wf (TRecord tl) ->
+        type_of_value (VRecord vl) (TRecord tl) ->
+        Forall2 (Datalog.interp_expr map.empty)
+          (map dexpr_literal
+             (map
+                (fun p => lower_atomic_value (snd p))
+                vl))
+          (map (fun p => lower_atomic_value (snd p))
+             vl).
+    Proof.
+      intros.
+      lazymatch goal with
+        H: type_wf _ |- _ => inversion H; subst; clear H
+      end; invert_type_of_value;
+      repeat lazymatch goal with
+          H: Forall2 _ (_ :: _) _ |- _ =>
+            inversion H; subst; clear H
+        end.
+      generalize dependent tl.
+      induction vl; cbn; constructor;
+        destruct tl; invert_Forall2.
+      1: destruct (snd a); cbn; econstructor; eauto.
+      1:{ cbn in *. invert_Forall.
+          repeat invert_Forall2.
+          invert_NoDup. invert_SSorted.
+          eapply IHvl; eauto. }
+    Qed.
+
+    Lemma lower_init_value_complete : forall x v t,
+        type_of_value v t ->
+        type_wf t ->
+        Forall
+          (fun vs =>
+             prog_impl_fact (lower_init_value (str_rel x) v)
+               (str_rel x, Zobj 0 :: vs))
+          (lower_value v).
+    Proof.
+      destruct 1; cbn.
+      1-3: repeat econstructor.
+      1:{ repeat econstructor.
+          eapply interp_expr__dexpr_literal_atomic; eauto.
+          constructor; auto. }
+      1:{ inversion 1; subst.
+          induction l; cbn; constructor.
+          1:{ repeat econstructor.
+              invert_Forall. instantiate (1:=map.empty).
+              lazymatch goal with
+                H: type_of_value _ _ |- _ =>
+                  inversion H; subst
+              end.
+              cbn.
+              eapply interp_expr__dexpr_literal_atomic; eauto. }
+          1:{ invert_Forall.
+              rewrite Forall_forall; intros.
+              eapply prog_impl_fact_weaken.
+              1:{ apply IHl in H5.
+                  apply_Forall_In. }
+              apply incl_tl, incl_refl. }
+          Unshelve. all: apply map.empty. }
+    Qed.
+
+    Lemma venv_is_lowered_to_at_0 : forall g_sig g_str rls,
+        sig_wf g_sig ->
+        str_wf (map snd g_sig) g_str ->
+        incl (concat
+                (map (fun '(x, v) => lower_init_value (str_rel x) v)
+                   (combine (map fst g_sig) g_str))) rls ->
+        venv_is_lowered_to_at (map fst g_sig) g_str rls 0.
+    Proof.
+      unfold str_wf, sig_wf. induction g_sig; cbn; intros;
+        invert_Forall2; constructor; cbn in *;
+        intuition idtac; invert_Forall; invert_NoDup.
+      1:{ unfold is_lowered_to_at.
+          rewrite Forall_forall.
+          intros.
+          lazymatch goal with
+            H: type_of_value _ _ |- _ =>
+              eapply lower_init_value_complete in H
+          end; trivial.
+          apply_Forall_In.
+          eapply prog_impl_fact_weaken; eauto.
+          eapply List.incl_app_bw_l; eassumption. }
+      1:{ apply IHg_sig; auto.
+          eapply List.incl_app_bw_r. eauto. }
+    Qed.
+
+    Theorem lower_cfg_complete' : forall (g : cfg) (Gstore : tenv) (g_d' : cfg_dynamic) dcls rls,
+        lower_cfg g = (dcls, rls) ->
+        Gstore = mk_tenv g.(sig_blks).(sig) ->
+        well_typed_cfg g ->
+        cfg_steps g.(sig_blks) g.(str_ptr) g_d' ->
+        let muts := map fst g.(sig_blks).(sig) in
+        match g_d'.(ptr) with
+        | Some n =>
+            exists ts, venv_is_lowered_to_at muts g_d'.(str) rls ts /\
+                         prog_impl_fact rls (blk_rel n, [Zobj ts])
+        | None => venv_is_lowered_to muts g_d'.(str) rls
+        end.
+    Proof.
+      unfold well_typed_cfg, lower_cfg; intros.
+      intuition idtac.
+      lazymatch goal with
+        H: context[cfg_steps] |- _ =>
+          induction H
+      end; intros.
+      1:{ repeat destruct_match_hyp; subst;
+          invert_pair.
+          1:{ exists 0%Z; split.
+              1:{ unfold sig_wf in *.
+                  apply venv_is_lowered_to_at_0; auto.
+                  apply incl_tl, incl_appl, incl_refl. }
+              1:{ econstructor.
+                  1:{ left. econstructor.
+                      repeat eexists; eauto;
+                        repeat econstructor. }
+                  trivial. } }
+          1:{ admit. } }
+      1:{ lazymatch goal with
+          H: context[cfg_step] |- _ =>
+            inversion H; subst
+        end.
+          repeat lazymatch goal with
+                   H: ?x = _, _: context[?x] |- _ =>
+                     rewrite H in *
+                 end.
+          repeat destruct_match_hyp; subst.
+    Admitted.
+
+
+    Theorem lower_cfg_sound : forall (g : cfg) (Gstore : tenv) (store : venv) dcls rls,
+        lower_cfg g = (dcls, rls) ->
+        Gstore = mk_tenv g.(sig) ->
+        well_typed_cfg g ->
+        cfg_impl g store ->
+        venv_is_lowered_from Gstore rls store.
+    Admitted.
   End WithVarenv.
 
-
 End __.
+Wanted to change the definitions of lower_aexpr and lower_pexpr and lower_rexpr to return via output relation, as their soundness lemmas now involve a separate set of rules from which we can deduce (str_rel x)[t; ...], and it's unclear how to talk about interp_fact and Datalog.interp_expr with respect to some "free relation" that's created in a separate set of rules.
+
+But cannot change because of the way relational algebra constructs are lowered: the assumption of variable names for accessing the attribute of a row only has the scope within a rule, and generating a rule for lower_aexpr / lower_pexpr won't do.
+
+
+                                                                                                                                                            entry a pointer                                                                                        relate v with sets of tuples
